Computability/SingleOracle/RecursiveInTheorems.lean
@@ -6,7 +6,6 @@ open Classical
 
 open Nat.RecursiveIn.Code
 
-
 @[simp] lemma Nat.RecursiveIn.partCompTotal {O:ℕ→ℕ} {f:ℕ→.ℕ} {g:ℕ→ℕ} (h1: Nat.RecursiveIn O f) (h2: Nat.RecursiveIn O g) : (Nat.RecursiveIn O ↑(f∘g)) := by
   have h3 : (↑(f∘g):ℕ→.ℕ) = fun x => g x >>= (↑f:ℕ→.ℕ) := by
     funext xs
@@ -24,6 +23,58 @@ open Nat.RecursiveIn.Code
   apply Nat.RecursiveIn.totalComp
   · exact h1
   · apply Nat.RecursiveIn.id
+
+
+
+namespace Nat.RecursiveIn.Code
+theorem exists_code_nat (O : ℕ → ℕ) (f : ℕ →. ℕ) : Nat.RecursiveIn O f ↔ ∃ c : ℕ , eval O c = f := by
+  have h {f : ℕ →. ℕ} : Nat.RecursiveIn O f ↔ ∃ c : Nat.RecursiveIn.Code, eval O c = f := by exact
+    exists_code
+  constructor
+  · intro h2
+    obtain ⟨c, h3⟩ := h.mp h2
+    use c.encodeCode
+    simp only [decodeCode_encodeCode]
+    exact h3
+  · intro h2
+    obtain ⟨c, h3⟩ := h2
+    have h5: (∃ c:Nat.RecursiveIn.Code, eval O c = f) := by
+      use decodeCode c
+    exact exists_code.mpr h5
+def eval₁ (O:ℕ→ℕ) : ℕ→.ℕ := fun ex => eval O ex.unpair.1 ex.unpair.2
+@[simp] theorem eval₁_rw_eval : eval₁ O = fun ex => eval O ex.unpair.1 ex.unpair.2 := by exact rfl
+theorem rec_eval₁ : Nat.RecursiveIn O (eval₁ O) := by
+  simp only [eval₁_rw_eval]
+  exact RecursiveIn.nat_iff.mp eval_part
+theorem exists_code_for_eval₁ : ∃ c:ℕ, eval O c = eval₁ O := by
+  apply ((exists_code_nat O (eval₁ O)).mp)
+  exact rec_eval₁
+
+
+theorem Nat.RecursiveIn.evalRecInO' {O} {f:ℕ→.ℕ} (h:Nat.RecursiveIn O f) : Nat.RecursiveIn O (fun x => (f x) >>= (eval₁ O)) := by
+  simp only [Part.bind_eq_bind]
+  refine _root_.Nat.RecursiveIn.comp ?_ h
+  apply rec_eval₁
+theorem Nat.RecursiveIn.eval_K_computable : Nat.RecursiveIn O (fun x ↦ eval O x x) := by
+  have h : (fun (x:ℕ) ↦ eval O x x) = (fun (x:ℕ) => eval O x.unpair.1 x.unpair.2) ∘ (fun x=>Nat.pair x x) := by
+    funext xs
+    simp only [Function.comp_apply, Nat.unpair_pair]
+  rw [h]
+  refine Nat.RecursiveIn.partCompTotal ?_ ?_
+  exact rec_eval₁
+  exact Nat.RecursiveIn.of_primrec (Nat.Primrec.pair Nat.Primrec.id Nat.Primrec.id)
+
+
+end Nat.RecursiveIn.Code
+
+
+
+
+
+
+
+
+
 
 
 @[simp] def Nat.flatten := fun x => if x=0 then 0 else 1
@@ -119,40 +170,6 @@ lemma Nat.Primrec.pair_proj : Nat.Primrec (Nat.pair x) := by
   exact Primrec₂.natPair
 
 
-def Nat.RecursiveIn.Code.eval' (O:ℕ→ℕ) : (ℕ→.ℕ) := fun y => (eval O) (y.unpair.1) (y.unpair.2)
--- def Nat.ComputableIn (O f : ℕ->ℕ) := Nat.RecursiveIn O f
-theorem RecursiveIn.eval_rec {O} : RecursiveIn O (eval' O) := by exact eval_part
-theorem Nat.RecursiveIn.eval_rec {O} : Nat.RecursiveIn O (eval' O) := by exact RecursiveIn.nat_iff.mp _root_.RecursiveIn.eval_rec
-
-theorem Nat.RecursiveIn.evalRecInO' {O} {f:ℕ→.ℕ} (h:Nat.RecursiveIn O f) : Nat.RecursiveIn O (fun x => (f x) >>= (eval' O)) := by
-  simp only [Part.bind_eq_bind]
-  refine comp ?_ h
-  apply Nat.RecursiveIn.eval_rec
-theorem Nat.RecursiveIn.eval_K_computable : Nat.RecursiveIn O (fun x ↦ eval O x x) := by
-  have h : (fun (x:ℕ) ↦ eval O x x) = (fun (x:ℕ) => eval O x.unpair.1 x.unpair.2) ∘ (fun x=>Nat.pair x x) := by
-    funext xs
-    simp only [Function.comp_apply, Nat.unpair_pair]
-  rw [h]
-  refine Nat.RecursiveIn.partCompTotal ?_ ?_
-  exact Nat.RecursiveIn.eval_rec
-  exact Nat.RecursiveIn.of_primrec (Nat.Primrec.pair Nat.Primrec.id Nat.Primrec.id)
-
-theorem exists_code_nat (O : ℕ → ℕ) (f : ℕ →. ℕ) : Nat.RecursiveIn O f ↔ ∃ c : ℕ , eval O c = f := by
-  have h {f : ℕ →. ℕ} : Nat.RecursiveIn O f ↔ ∃ c : Nat.RecursiveIn.Code, eval O c = f := by exact
-    exists_code
-  constructor
-  · intro h2
-    obtain ⟨c, h3⟩ := h.mp h2
-    use c.encodeCode
-    simp only [decodeCode_encodeCode]
-    exact h3
-  · intro h2
-    obtain ⟨c, h3⟩ := h2
-    have h5: (∃ c:Nat.RecursiveIn.Code, eval O c = f) := by
-      use decodeCode c
-    exact exists_code.mpr h5
-
-
 
 -- theorem smn_calc : ∃ f : ℕ → ℕ, ComputableIn O f ∧ ∀ c n random:ℕ, eval O (f ex) random = eval O ex.unpair.1 ex.unpair.2 :=
 --   by
@@ -168,14 +185,14 @@ theorem Nat.RecursiveIn.ite {O:ℕ→ℕ} {f g : ℕ→.ℕ} {c:ℕ→ℕ} (hc :
     rcases exists_index_for_f with ⟨index_f,index_f_is_f⟩
     rcases exists_index_for_g with ⟨index_g,index_g_is_g⟩
 
-    have main2 : (fun a => if (c a=0) then (f a) else (g a)) = fun a => Nat.pair (if c a=0 then (index_f) else (index_g)) a >>= eval' O := by
+    have main2 : (fun a => if (c a=0) then (f a) else (g a)) = fun a => Nat.pair (if c a=0 then (index_f) else (index_g)) a >>= eval₁ O := by
       funext xs
       cases Classical.em (c xs = 0) with
       | inl h =>
-        simp only [h, ↓reduceIte, Part.coe_some, Part.bind_eq_bind, Part.bind_some, eval', Nat.unpair_pair]
+        simp only [h, ↓reduceIte, Part.coe_some, Part.bind_eq_bind, Part.bind_some, eval₁, Nat.unpair_pair]
         exact congrFun (_root_.id (Eq.symm index_f_is_f)) xs
       | inr h =>
-        simp only [h, ↓reduceIte, Part.coe_some, Part.bind_eq_bind, Part.bind_some, eval', Nat.unpair_pair]
+        simp only [h, ↓reduceIte, Part.coe_some, Part.bind_eq_bind, Part.bind_some, eval₁, Nat.unpair_pair]
         exact congrFun (_root_.id (Eq.symm index_g_is_g)) xs
     rw [main2]
 
